Steps.thy
@@ -11,9 +11,10 @@ datatype instruction_state = execi "llvm_identifier option" llvm_instruction_blo
   | flowi state llvm_block_return
   | is_erri: erri
 
-datatype (discs_sels) function_state = branchf (state: state) "llvm_identifier option" "llvm_identifier" llvm_function
-  | retf (state: state) (ret_value: "llvm_value option")
+datatype (discs_sels) function_state = branchf (state: state) "llvm_identifier option" llvm_identifier llvm_identifier
+  | retf (state: state) (ret_value: "llvm_value option") llvm_identifier
   | is_errf: errf 
+definition "first_label f \<equiv> (case llvm_function.blocks f of ((l,b)#fs) \<Rightarrow> Some l | _ \<Rightarrow> None)"
 
 
 inductive
@@ -35,6 +36,12 @@ where
 | "get_register s v = err _ \<Longrightarrow>
     (execi pre ([],[],ret (Some (t, v))) s) \<rightarrow>\<^sub>i erri"
 
+(*
+| "map_of (funcs program) f = Some fu
+  \<Longrightarrow> first_label fu = Some b
+  \<Longrightarrow> step_f\<^sup>*\<^sup>* (branchf (new_frame s) None b fu) (retf s' v')
+  \<Longrightarrow> (execi pre ([],(call n ty f p)#is,t) s) \<rightarrow>\<^sub>i (execi pre ([],is,t) (restore_frame s s'))"
+*)
 | "execute_instruction i s = ok s' \<Longrightarrow>
     (execi pre ([],i#is,t) s) \<rightarrow>\<^sub>i (execi pre ([],is,t) s')"
 | "execute_instruction i s = err _ \<Longrightarrow>
@@ -45,17 +52,23 @@ where
 | "execute_phi pre p s = err _ \<Longrightarrow>
     (execi pre (p#ps,is,t) s) \<rightarrow>\<^sub>i erri"
 
-| "map_of (llvm_function.blocks f) lab = Some b \<Longrightarrow>
-   step_i\<^sup>*\<^sup>* (execi prev b s) (flowi s' (branch_label l)) \<Longrightarrow>
-     branchf s prev lab f \<rightarrow>\<^sub>f branchf s' (Some lab) l f"
-| "map_of (llvm_function.blocks f) lab = Some b \<Longrightarrow>
-   step_i\<^sup>*\<^sup>* (execi prev b s) (flowi s' (return_value v)) \<Longrightarrow>
-     branchf s prev lab f \<rightarrow>\<^sub>f retf s' v"
+| "map_of (funcs program) f = Some fu \<Longrightarrow>
+    map_of (llvm_function.blocks fu) lab = Some b \<Longrightarrow>
+    step_i\<^sup>*\<^sup>* (execi prev b s) (flowi s' (branch_label l)) \<Longrightarrow>                                                          
+    branchf s prev lab f \<rightarrow>\<^sub>f branchf s' (Some lab) l f"
+| "map_of (funcs program) f = Some fu \<Longrightarrow>
+    map_of (llvm_function.blocks fu) lab = Some b \<Longrightarrow>
+    step_i\<^sup>*\<^sup>* (execi prev b s) (flowi s' (return_value v)) \<Longrightarrow>
+    branchf s prev lab f \<rightarrow>\<^sub>f retf s' v f"
 
-| "map_of (llvm_function.blocks f) lab = Some b \<Longrightarrow>
-   step_i\<^sup>*\<^sup>* (execi prev b s) erri \<Longrightarrow>
+| "map_of (funcs program) f = Some fu \<Longrightarrow>
+    map_of (llvm_function.blocks fu) lab = Some b \<Longrightarrow>
+    step_i\<^sup>*\<^sup>* (execi prev b s) erri \<Longrightarrow>
+    branchf s prev lab f \<rightarrow>\<^sub>f errf"
+| "map_of (funcs program) f = Some fu \<Longrightarrow>
+    map_of (llvm_function.blocks fu) lab = None \<Longrightarrow>
      branchf s prev lab f \<rightarrow>\<^sub>f errf"
-| "map_of (llvm_function.blocks f) lab = None \<Longrightarrow>
+| "map_of (funcs program) f = None \<Longrightarrow>
      branchf s prev lab f \<rightarrow>\<^sub>f errf"
 
 
@@ -74,18 +87,17 @@ fun n_steps_f :: "function_state \<Rightarrow> nat \<Rightarrow> function_state 
 notation n_steps_i ("(_ \<rightarrow>\<^sub>i^_ _)" [51, 0, 51] 50)
 notation n_steps_f ("(_ \<rightarrow>\<^sub>f^_ _)" [51, 0, 51] 50)
 
+
 lemma steps_i_exists_n_steps[simp]:
   assumes "fs \<rightarrow>\<^sub>i* fs'"
   shows "\<exists>n. fs \<rightarrow>\<^sub>i^n fs'"
   using assms n_steps_i.simps
   by (induction rule: converse_rtranclp_induct; blast)
-
 lemma steps_f_exists_n_steps[simp]:
   assumes "fs \<rightarrow>\<^sub>f* fs'"
   shows "\<exists>n. fs \<rightarrow>\<^sub>f^n fs'"
   using assms n_steps_f.simps
   by (induction rule: converse_rtranclp_induct; blast)
-
 
 definition terminal_state_i where
   "terminal_state_i s \<equiv> \<nexists>s'. s \<rightarrow>\<^sub>i s'"
@@ -95,16 +107,13 @@ definition terminal_state_f where
 notation terminal_state_i ("_ \<nexists>\<rightarrow>\<^sub>i" 50)
 notation terminal_state_f ("_ \<nexists>\<rightarrow>\<^sub>f" 50)
 
-
-definition "first_label f \<equiv> (case llvm_function.blocks f of ((l,b)#fs) \<Rightarrow> Some l | _ \<Rightarrow> None)"
-
-
 lemma term_state_i_simps[simp]:
   "\<not> ((execi pre b s) \<nexists>\<rightarrow>\<^sub>i)"
   "(flowi s br) \<nexists>\<rightarrow>\<^sub>i"
   "erri \<nexists>\<rightarrow>\<^sub>i"
     apply clarsimp
-  apply (cases b; cases s)
+    apply (cases b; cases s)
+  
   subgoal for phis instrs ter l g s h
     unfolding terminal_state_i_def
     apply (cases phis; cases instrs; cases ter)
@@ -175,16 +184,19 @@ lemma step_i_reaches_term_state:
 
 lemma term_state_f_simps[simp]:
   "errf \<nexists>\<rightarrow>\<^sub>f"
-  "retf s v \<nexists>\<rightarrow>\<^sub>f"
+  "retf s v f \<nexists>\<rightarrow>\<^sub>f"
   "\<not> ((branchf s prev lab f) \<nexists>\<rightarrow>\<^sub>f)"
   unfolding terminal_state_f_def
     apply simp
   using step_f.cases apply blast
   using step_f.cases apply blast
-  apply (cases "map_of (llvm_function.blocks f) lab")
+  apply (cases "map_of (funcs program) f") 
+  using step_i_step_f.intros(15) apply blast
+  subgoal for fu
+  apply (cases "map_of (llvm_function.blocks fu) lab")
   using step_i_step_f.intros(14) apply blast
   subgoal premises prems for b
-  proof (cases "execi prev b s \<rightarrow>\<^sub>i*  erri")
+  proof (cases "execi prev b s \<rightarrow>\<^sub>i* erri")
     case True
     then show ?thesis
       using step_i_step_f.intros(13) prems
@@ -205,7 +217,7 @@ lemma term_state_f_simps[simp]:
       by (cases br; meson)
   qed
   done
-
+  done
 
 
 lemma steps_model_exec:
@@ -274,115 +286,47 @@ lemma single_step_eq_exec_step:
   by fastforce
 
 
-lemma step_i_deterministic[simp]:
-  assumes "s \<rightarrow>\<^sub>i s1"
-  assumes "s \<rightarrow>\<^sub>i s2"
+find_theorems "x = y \<Longrightarrow> y = x"
+
+thm step_i_step_f.induct
+thm step_i_step_f.inducts
+
+lemma steps_i_deter:
+  "st \<rightarrow>\<^sub>i* st' \<Longrightarrow> st' \<nexists>\<rightarrow>\<^sub>i \<Longrightarrow> st \<rightarrow>\<^sub>i* st'' \<Longrightarrow> st'' \<nexists>\<rightarrow>\<^sub>i \<Longrightarrow> st' = st''"
+        apply (induction rule: converse_rtranclp_induct)
+         apply (metis terminal_state_i_def converse_rtranclpE)
+        by (smt (verit) converse_rtranclpE instruction_state.sel(1,2,3) list.discI list.inject
+            llvm_terminator_instruction.distinct(1,3,5) llvm_terminator_instruction.inject(1,2,3) llvm_value.inject(1)
+            option.distinct(1) option.simps(1) prod.inject result.distinct(1) result.inject(1) step_i.cases
+            term_state_i_simps(1))
+lemma
+  assumes "(\<lambda>s s'. R s s' \<and> (\<forall>s''. R s s'' \<longrightarrow> s' = s''))\<^sup>*\<^sup>* s s1 \<and> (\<nexists>s'. (\<lambda>s s'. R s s' \<and> (\<forall>s''. R s s'' \<longrightarrow> s' = s'')) s1 s')"
+  assumes "(\<lambda>s s'. R s s' \<and> (\<forall>s''. R s s'' \<longrightarrow> s' = s''))\<^sup>*\<^sup>* s s2 \<and> (\<nexists>s'. (\<lambda>s s'. R s s' \<and> (\<forall>s''. R s s'' \<longrightarrow> s' = s'')) s2 s')"
   shows "s1 = s2"
-proof -
-  show ?thesis
-    using assms
-    apply (cases s)
-    apply (smt (verit) Pair_inject instruction_state.inject(1) list.discI
-        llvm_terminator_instruction.distinct(3,5) llvm_terminator_instruction.inject(3)
-        step_i.cases)
-    
-    apply (smt (verit) instruction_state.inject(1) list.discI llvm_terminator_instruction.distinct(1,5)
-        llvm_terminator_instruction.inject(2) llvm_value.inject(1) prod.inject result.inject(1)
-        step_i.cases)
+  using assms apply auto
+        apply (induction arbitrary: s2 rule: converse_rtranclp_induct)
+  using converse_rtranclpE
+  apply (smt (verit, ccfv_threshold))
+  using converse_rtranclpE
+  apply (smt (verit, ccfv_threshold))
+  done
 
-    apply (smt (verit) Pair_inject instruction_state.inject list.discI
-        llvm_terminator_instruction.distinct llvm_terminator_instruction.inject
-        step_i.cases)
-    
-    apply (smt (verit, ccfv_SIG) Pair_inject instruction_state.inject(1) list.discI
-        llvm_terminator_instruction.distinct(1,3) llvm_terminator_instruction.inject(1) option.distinct(1)
-        step_i.cases)
-
-    defer
-         defer
-    apply (smt (verit, ccfv_SIG) fst_conv instruction_state.sel(1,2,3) list.discI list.inject
-        result.distinct(1) result.inject(1) snd_conv step_i.cases)
-    apply (smt (verit, ccfv_SIG) fst_conv instruction_state.sel(1,2,3) list.discI list.inject
-        result.distinct(1) result.inject(1) snd_conv step_i.cases)
-    apply (smt (verit, ccfv_SIG) fst_conv instruction_state.sel(1,2,3) list.discI list.inject
-        result.distinct(1) result.inject(1) snd_conv step_i.cases)
-    apply (smt (verit, ccfv_SIG) fst_conv instruction_state.sel(1,2,3) list.discI list.inject
-        result.distinct(1) result.inject(1) snd_conv step_i.cases)
-    subgoal premises prems for stat v v' pre t
-    proof (cases s2)
-      case (execi x11 x12 x13)
-      then show ?thesis
-        using prems
-        by (smt (verit) instruction_state.distinct(1,4) instruction_state.sel(2) list.discI prod.inject
-          step_i.cases)
-    next
-      case (flowi st br)
-
-      then obtain val where brdef: "br = return_value (Some val)"
-        using prems Pair_inject instruction_state.distinct(1,6) instruction_state.inject(1,2)
-            llvm_terminator_instruction.distinct(1,3) step_i.cases
-        by (smt (verit, ccfv_SIG) llvm_terminator_instruction.inject(1) option.distinct(1))
-
-      then have "get_register stat v = ok val"
-        using prems flowi step_i.cases
-        by blast
-
-      then show ?thesis                        
-        using brdef flowi prems(1,2,3,4) step_i.cases by auto
-    next
-      case erri
-      have "\<forall>e. get_register stat v \<noteq> err e" using prems by simp
-      then have "\<not>s \<rightarrow>\<^sub>i erri" using prems step_i.cases by blast
-      then show ?thesis using prems erri by blast
-    qed
-  subgoal premises prems for stat v v' pre t
-    proof (cases s2)
-      case (execi x11 x12 x13)
-      then show ?thesis
-        using prems
-        by (smt (verit) instruction_state.distinct(1,4) instruction_state.sel(2) list.discI prod.inject
-          step_i.cases)
-    next
-      case (flowi st br)
-
-      then obtain val where brdef: "br = return_value (Some val)"
-        using prems Pair_inject instruction_state.distinct(1,6) instruction_state.inject(1,2)
-            llvm_terminator_instruction.distinct(1,3) step_i.cases
-        by (smt (verit, ccfv_SIG) llvm_terminator_instruction.inject(1) option.distinct(1))
-
-      then have "get_register stat v = ok val"
-        using prems flowi step_i.cases
-        by blast
-
-      then show ?thesis                        
-        using brdef flowi prems(1,2,3,4) step_i.cases by auto
-    next
-      case erri
-      have "\<forall>e. get_register stat v \<noteq> ok e" using prems by simp
-      then show ?thesis using prems erri by blast
-    qed
-    done
-qed
-
-lemma step_f_deterministic[simp]:
-  assumes "s \<rightarrow>\<^sub>f s1"
-  assumes "s \<rightarrow>\<^sub>f s2"
-  shows "s1 = s2"
-proof (cases s)
-  case (branchf s prev lab f)
-  then show ?thesis sorry
-next
-  case (retf x21 x22)
-  then show ?thesis
-    using assms
-    by (metis term_state_f_simps(2) terminal_state_f_def)
-next
-  case errf
-  then show ?thesis
-    using assms
-    by (metis term_state_f_simps(1) terminal_state_f_def)
-qed
-
+lemma step_deterministic[simp]:
+  "si \<rightarrow>\<^sub>i si1 \<Longrightarrow> si \<rightarrow>\<^sub>i si2 \<Longrightarrow> si1 = si2"
+  "sf \<rightarrow>\<^sub>f sf1 \<Longrightarrow> sf \<rightarrow>\<^sub>f sf2 \<Longrightarrow> sf1 = sf2"
+  apply (induction arbitrary: si2 rule: step_i_step_f.inducts)
+               apply (auto simp add: step_i.simps)[10]
+  apply (smt (verit, best) function_state.sel(1,3,4,5) instruction_state.distinct(6) instruction_state.inject(2)
+          llvm_block_return.distinct(1) llvm_block_return.inject(2) mono_rtranclp option.distinct(1) option.sel
+          step_f.cases term_state_i_simps(2,3) steps_i_deter) 
+  apply (smt (verit, best) function_state.sel instruction_state.distinct instruction_state.inject
+          llvm_block_return.distinct(1) llvm_block_return.inject mono_rtranclp option.distinct(1) option.sel
+          step_f.cases term_state_i_simps steps_i_deter)
+  apply (smt (verit, best) function_state.sel instruction_state.distinct instruction_state.inject
+          llvm_block_return.distinct(1) llvm_block_return.inject mono_rtranclp option.distinct(1) option.sel
+          step_f.cases term_state_i_simps steps_i_deter)
+  using step_f.cases apply fastforce
+  using step_f.cases by fastforce
 
 definition "wp_instrs s Q \<equiv> \<forall>s'. s \<rightarrow>\<^sub>i* s' \<and> terminal_state_i s' \<longrightarrow> \<not>is_erri s' \<and> Q s'"
 
@@ -434,10 +378,10 @@ lemma block_ret_Some_wp_intro[wp_instrs_intro]:
   subgoal premises prems for s'
     proof -
       have "(execi pre ([], [], ret (Some (type, value))) s) \<rightarrow>\<^sub>i (flowi s (return_value (Some v)))"
-        using prems step_i.intros register_\<alpha>_eq_get_register
+        using prems step_i_step_f.intros register_\<alpha>_eq_get_register
         by auto
 
-        then show ?thesis using step_i_deterministic
+        then show ?thesis using step_deterministic
           by (smt (verit, ccfv_SIG)
               converse_rtranclpE instruction_state.distinct(6) is_erri_def prems(2,3,4) step_i.cases
               term_state_i_simps(1,2))
@@ -453,10 +397,10 @@ lemma block_ret_None_wp_intro[wp_instrs_intro]:
   subgoal premises prems for s'
     proof -
       have "step_i (execi pre ([], [], ret None) s) (flowi s (return_value None))"
-        using prems step_i.intros
+        using prems step_i_step_f.intros
         by auto
 
-        then show ?thesis using step_i_deterministic
+        then show ?thesis using step_deterministic
           by (smt (verit, ccfv_SIG)
               converse_rtranclpE instruction_state.distinct(6) is_erri_def prems step_i.cases
               term_state_i_simps(1,2))
@@ -488,304 +432,114 @@ lemma block_br_i1_wp_intro[wp_instrs_intro]:
 
 
 
-
-lemma terminal_state_simps[simp]: 
-  "terminal_state berr"
-  "terminal_state (bret s v)"
-  "\<not>terminal_state (bbranch s prev lab)"
-  unfolding terminal_state_def
-    apply auto apply (cases "map_of (llvm_function.blocks f) lab"; simp)
-  subgoal for b
-    apply (cases b)
-    subgoal premises prems for phis instrs ter
-      using prems(2)
-    proof (induction phis arbitrary: b s)
-      case phinil: Nil
-      then show ?case
-      proof (induction instrs arbitrary: b s)
-        case insnil: Nil
-        then show ?case
-        proof(cases ter)
-          case (ret x1)
-          then show ?thesis
-          proof (cases x1)
-            case None
-            then show ?thesis by (metis (mono_tags, lifting) ret instruction_state.simps(10) llvm_block_return.simps(5) insnil r_into_rtranclp
-                step_i.intros(4) term_state_i_simps(2))
-          next
-            case (Some v)
-            then obtain s' where "execi prev ([],[],ter) s \<rightarrow>\<^sub>i s'"
-              using term_state_i_simps unfolding terminal_state_i_def by meson
-            then have "s' = erri \<or> (\<exists>s'' v'. s' = flowi s'' v')"
-              by (smt (verit) instruction_state.inject(1) list.discI list.inject prod.inject
-                  step_i.cases)
-            then have "\<exists>ss' ss. step_i\<^sup>*\<^sup>* s' ss \<and> terminal_state_i ss \<and>
-            (case ss of flowi stat (return_value v) \<Rightarrow> ss' = bret stat v
-              | flowi stat (branch_label l) \<Rightarrow> ss' = bbranch stat (Some lab) l | erri \<Rightarrow> ss' = berr)"
-                using prems phinil insnil ret Some
-                by (metis (mono_tags, lifting) instruction_state.simps(10,11) llvm_block_return.exhaust llvm_block_return.simps(5,6)
-                    rtranclp.simps term_state_i_simps(2,3))
-
-            then show ?thesis using prems phinil insnil ret Some
-              by (metis (no_types, lifting) \<open>execi prev ([], [], ter) s \<rightarrow>\<^sub>i s'\<close> converse_rtranclp_into_rtranclp)
-          qed
-        next
-          case (br_i1 x21 x22 x23)
-            then obtain s' where "execi prev ([],[],ter) s \<rightarrow>\<^sub>i s'"
-              using term_state_i_simps unfolding terminal_state_i_def by meson
-            then have "s' = erri \<or> (\<exists>s'' v'. s' = flowi s'' v')"
-              by (smt (verit) instruction_state.inject(1) list.discI list.inject prod.inject
-                  step_i.cases)
-            then have "\<exists>ss' ss. step_i\<^sup>*\<^sup>* s' ss \<and> terminal_state_i ss \<and>
-            (case ss of flowi stat (return_value v) \<Rightarrow> ss' = bret stat v
-              | flowi stat (branch_label l) \<Rightarrow> ss' = bbranch stat (Some lab) l | erri \<Rightarrow> ss' = berr)"
-                using prems phinil insnil br_i1
-                by (metis (mono_tags, lifting) instruction_state.simps(10,11) llvm_block_return.exhaust llvm_block_return.simps(5,6)
-                    rtranclp.simps term_state_i_simps(2,3))
-          then show ?thesis using prems phinil insnil
-              by (metis (no_types, lifting) \<open>execi prev ([], [], ter) s \<rightarrow>\<^sub>i s'\<close> converse_rtranclp_into_rtranclp)
-        next
-          case (br_label x3)
-            then obtain s' where "execi prev ([],[],ter) s \<rightarrow>\<^sub>i s'"
-              using term_state_i_simps unfolding terminal_state_i_def by meson
-            then have "s' = erri \<or> (\<exists>s'' v'. s' = flowi s'' v')"
-              by (smt (verit) instruction_state.inject(1) list.discI list.inject prod.inject
-                  step_i.cases)
-            then have "\<exists>ss' ss. step_i\<^sup>*\<^sup>* s' ss \<and> terminal_state_i ss \<and>
-            (case ss of flowi stat (return_value v) \<Rightarrow> ss' = bret stat v
-              | flowi stat (branch_label l) \<Rightarrow> ss' = bbranch stat (Some lab) l | erri \<Rightarrow> ss' = berr)"
-                using prems phinil insnil br_label
-                by (metis (mono_tags, lifting) instruction_state.simps(10,11) llvm_block_return.exhaust llvm_block_return.simps(5,6)
-                    rtranclp.simps term_state_i_simps(2,3))
-          then show ?thesis using prems phinil insnil
-              by (metis (no_types, lifting) \<open>execi prev ([], [], ter) s \<rightarrow>\<^sub>i s'\<close> converse_rtranclp_into_rtranclp)
-        qed
-      next
-        case (Cons i ins)
-
-        then obtain s' where "execi prev ([],i#ins,ter) s \<rightarrow>\<^sub>i s'"
-          using term_state_i_simps unfolding terminal_state_i_def by meson
-
-        then have "s'= erri \<or> (\<exists>st. s' = execi prev ([],ins,ter) st)"
-          by (smt (verit) instruction_state.inject(1) list.discI list.inject prod.inject
-            step_i.cases)
-      then have "\<exists>ss' ss. step_i\<^sup>*\<^sup>* s' ss \<and> terminal_state_i ss \<and>
-       (case ss of flowi stat (return_value v) \<Rightarrow> ss' = bret stat v
-        | flowi stat (branch_label l) \<Rightarrow> ss' = bbranch stat (Some lab) l | erri \<Rightarrow> ss' = berr)"
-        using prems Cons Nil by fastforce
-
-        then show ?case using prems Cons.IH
-          by (metis (no_types, lifting) Cons.prems \<open>execi prev ([], i # ins, ter) s \<rightarrow>\<^sub>i s'\<close> converse_rtranclp_into_rtranclp)
-      qed
-        
-    next
-      case (Cons p ps b s)
-      
-      then obtain s' where "(execi prev (p#ps,instrs,ter) s) \<rightarrow>\<^sub>i s'"
-        using term_state_i_simps unfolding terminal_state_i_def by meson
-
-      then have "s' = erri \<or> (\<exists>st. s' = execi prev (ps,instrs,ter) st)"
-        by (smt (verit) instruction_state.inject(1) list.discI list.inject prod.inject
-            step_i.cases)
-        
-
-      then have "\<exists>ss' ss. step_i\<^sup>*\<^sup>* s' ss \<and> terminal_state_i ss \<and>
-       (case ss of flowi stat (return_value v) \<Rightarrow> ss' = bret stat v
-        | flowi stat (branch_label l) \<Rightarrow> ss' = bbranch stat (Some lab) l | erri \<Rightarrow> ss' = berr)"
-        using prems Cons by fastforce
-
-      then show ?case using prems Cons.IH
-        by (metis (no_types, lifting) Cons.prems \<open>step_i (execi prev (p # ps, instrs, ter) s) s'\<close>
-            converse_rtranclp_into_rtranclp)
-      qed
-          done done 
-
 lemma terminal_steps_refl[simp]:
-  "terminal_state s \<Longrightarrow> s \<rightarrow>* s' \<longleftrightarrow> s'=s"
-  unfolding terminal_state_def
+  "sf \<nexists>\<rightarrow>\<^sub>f \<Longrightarrow> sf \<rightarrow>\<^sub>f* sf' \<longleftrightarrow> sf'=sf"
+  "si \<nexists>\<rightarrow>\<^sub>i \<Longrightarrow> si \<rightarrow>\<^sub>i* si' \<longleftrightarrow> si'=si"
+  unfolding terminal_state_f_def terminal_state_i_def
   by (auto elim: converse_rtranclpE)
 
 lemma terminal_non_err[simp]:
-  "terminal_state s \<and> \<not>is_berr s \<longleftrightarrow> is_bret s"
+  "s \<nexists>\<rightarrow>\<^sub>f \<and> \<not>is_errf s \<longleftrightarrow> is_retf s"
   by (cases s; auto)
 
-lemma step_deterministic[simp]:
-  "is_bbranch fs \<Longrightarrow> \<exists>fs'. step fs fs'"
-  "is_bbranch fs \<Longrightarrow> \<nexists>fs' fs''. step fs fs' \<and> step fs fs'' \<and> fs' \<noteq> fs''"
-  apply auto
-  using terminal_non_err terminal_state_def apply blast
-  apply (cases fs)
-    apply simp_all
-  subgoal for fs' fs'' s prev l
-    apply (cases "map_of (llvm_function.blocks f) l")
-     apply simp_all
-      apply (elim exE conjE)
-    subgoal premises prems for b ss' ss''
-    proof -
-      obtain n where ndef: "execi prev b s \<rightarrow>\<^sub>i^n ss'"
-        using prems
-        by fastforce
-
-      moreover
-
-      obtain m where mdef: "execi prev b s \<rightarrow>\<^sub>i^m ss''"
-        using prems
-        by fastforce
-
-      ultimately
-
-      show ?thesis
-      proof (induction n arbitrary: prev b s m)
-        case 0
-        then show ?case using prems by auto
-      next
-        case nsuc: (Suc n')
-        then show ?case
-        proof (induction m arbitrary: prev b s)
-          case 0
-          then show ?case using prems by auto
-        next
-          case (Suc m')
-          
-          obtain s' where nextstate: "execi prev b s \<rightarrow>\<^sub>i s'"
-            using term_state_i_simps(1) terminal_state_i_def by blast
-
-          have nextmsteps: "s' \<rightarrow>\<^sub>i^m' ss''" using nextstate Suc
-            by (metis n_steps_i.simps(2) step_i_deterministic)
-
-          moreover
-
-          have nextnsteps: "s' \<rightarrow>\<^sub>i^n' ss'" using nextstate Suc
-            by (metis n_steps_i.simps(2) step_i_deterministic)
-
-          ultimately
-          
-          show ?case
-          proof(cases s')
-            case (execi x11 x12 x13)
-            then show ?thesis using nextmsteps nextnsteps nextstate Suc nsuc by blast  
-          next
-            case (flowi x21 x22)
-
-            have "m' = 0" using nextmsteps flowi
-              by (meson n_steps_i.elims(1) term_state_i_simps(2) terminal_state_i_def)
-
-            moreover
-
-            have "n' = 0" using nextnsteps flowi 
-              by (meson n_steps_i.elims(1) term_state_i_simps(2) terminal_state_i_def)
-
-            ultimately
-
-            have "ss' = ss''"using nextmsteps nextnsteps nextstate flowi prems Suc nsuc by simp
-            
-            then show ?thesis
-              using prems(6) prems(7) prems(8)
-              by (auto split: instruction_state.splits llvm_block_return.splits)
-          next
-            case erri
-            then show ?thesis
-              by (metis (mono_tags, lifting) instruction_state.simps(11) n_steps_i.elims(2) nextmsteps nextnsteps prems(6,8) term_state_i_simps(3) terminal_state_i_def)
-          qed
-        qed
-      qed
-    qed
-    done
-  done
-
-
-definition "wp_steps fs Q \<equiv> \<forall>fs'. fs \<rightarrow>* fs' \<and> terminal_state fs' \<longrightarrow> (\<not>is_berr fs') \<and> (Q (state fs') (ret_value fs'))"
+definition "wp_func fs Q \<equiv> \<forall>fs'. fs \<rightarrow>\<^sub>f* fs' \<and> (fs' \<nexists>\<rightarrow>\<^sub>f) \<longrightarrow> (\<not>is_errf fs') \<and> (Q (state fs') (ret_value fs'))"
 
 
 type_synonym precondition  = "state \<Rightarrow> bool"
 type_synonym preconditions = "((llvm_identifier option * llvm_identifier) * precondition) list"
 type_synonym postcondition = "state \<Rightarrow> llvm_value option \<Rightarrow> bool"
+type_synonym annotations = "(llvm_identifier * (preconditions * postcondition)) list"
 
-fun predicate_for_all where
-  "predicate_for_all P [] = True"
-| "predicate_for_all P (((p,l),pre)#pres) = (P p l \<and> predicate_for_all P pres)"
+
 
 context
-  fixes annotations :: "preconditions"
-  fixes post :: "postcondition"
+  fixes annotations :: "annotations"
 begin
-
-
-
-lemma
-  assumes "\<forall>fs'. fs \<rightarrow>* fs' \<and> terminal_state fs' \<longrightarrow> \<not>is_berr fs' \<and> post (state fs') (ret_value fs')"
-  shows "wp_steps fs post"
-  unfolding wp_steps_def using assms by blast
-
 
 definition "has_annotation fs \<equiv>
   (case fs of
-    berr \<Rightarrow> False
-  | bret _ _ \<Rightarrow> True
-  | bbranch _ p l \<Rightarrow> map_of annotations (p,l) \<noteq> None
+    errf \<Rightarrow> False
+  | retf _ _ f \<Rightarrow> map_of (funcs program) f \<noteq> None \<and> map_of annotations f \<noteq> None
+  | branchf _ p l f \<Rightarrow> map_of (funcs program) f \<noteq> None \<and>
+      (case map_of annotations f of 
+        None \<Rightarrow> False
+      | Some (pres,post) \<Rightarrow> map_of pres (p,l) \<noteq> None
+      )
   )"
 
 definition "annotation_holds fs \<equiv>
   (case fs of
-    berr \<Rightarrow> False
-  | bret s v \<Rightarrow> post s v
-  | bbranch s p l \<Rightarrow> 
-    (case map_of annotations (p,l) of
-      None \<Rightarrow> False
-    | Some annot \<Rightarrow> annot s
-    )
+    errf \<Rightarrow> False
+  | retf s v f \<Rightarrow> map_of (funcs program) f \<noteq> None \<and>
+      (case map_of annotations f of 
+        None \<Rightarrow> False
+      | Some (pres,post) \<Rightarrow> post s v
+      )
+  | branchf s p l f \<Rightarrow> map_of (funcs program) f \<noteq> None \<and>
+      (case map_of annotations f of 
+        None \<Rightarrow> False
+      | Some (pres,post) \<Rightarrow>
+          (case map_of pres (p,l) of
+            None \<Rightarrow> False
+          | Some pre \<Rightarrow> pre s
+          )
+      )
   )"
 
 
-definition step_until :: "flow_state \<Rightarrow> flow_state \<Rightarrow> bool" where
-  "step_until fs fs' \<equiv> step fs fs' \<and> \<not>has_annotation fs"
+definition step_until :: "function_state \<Rightarrow> function_state \<Rightarrow> bool" where
+  "step_until fs fs' \<equiv> fs \<rightarrow>\<^sub>f fs' \<and> \<not>has_annotation fs"
 
-definition annotated_step :: "flow_state \<Rightarrow> flow_state \<Rightarrow> bool" (infix "\<Rightarrow>" 50) where
-  "annotated_step s s' \<equiv> (\<exists>x. s \<rightarrow> x \<and> step_until\<^sup>*\<^sup>* x s') \<and> (has_annotation s' \<or> is_berr s')"
-abbreviation annotated_steps :: "flow_state \<Rightarrow> flow_state \<Rightarrow> bool" (infix "\<Rightarrow>*" 50) where
-  "fs \<Rightarrow>* fs' \<equiv> annotated_step\<^sup>*\<^sup>* fs fs'"
+definition annotated_step :: "function_state \<Rightarrow> function_state \<Rightarrow> bool" (infix "\<Rightarrow>\<^sub>f" 50) where
+  "s \<Rightarrow>\<^sub>f s' \<equiv> (\<exists>x. s \<rightarrow>\<^sub>f x \<and> step_until\<^sup>*\<^sup>* x s') \<and> (has_annotation s' \<or> is_errf s')"
+abbreviation annotated_steps :: "function_state \<Rightarrow> function_state \<Rightarrow> bool" (infix "\<Rightarrow>\<^sub>f*" 50) where
+  "fs \<Rightarrow>\<^sub>f* fs' \<equiv> annotated_step\<^sup>*\<^sup>* fs fs'"
 
 
 
 definition wp_step where
-  "wp_step fs Q \<equiv> (\<forall>fs'. step fs fs' \<longrightarrow> \<not>is_berr fs' \<and> Q fs')"
+  "wp_step fs Q \<equiv> (\<forall>fs'. fs \<rightarrow>\<^sub>f fs' \<longrightarrow> \<not>is_errf fs' \<and> Q fs')"
 
 definition wp_steps_until where
-  "wp_steps_until fs Q \<equiv> (\<forall>fs'. (step_until)\<^sup>*\<^sup>* fs fs' \<and> \<not>is_berr fs \<longrightarrow> \<not>is_berr fs') \<and> (\<forall>fs'. (step_until)\<^sup>*\<^sup>* fs fs' \<and> has_annotation fs' \<longrightarrow> Q fs')"
+  "wp_steps_until fs Q \<equiv> (\<forall>fs'. (step_until)\<^sup>*\<^sup>* fs fs' \<and> \<not>is_errf fs \<longrightarrow> \<not>is_errf fs') \<and> (\<forall>fs'. (step_until)\<^sup>*\<^sup>* fs fs' \<and> has_annotation fs' \<longrightarrow> Q fs')"
 
 definition wp_annotated_step where
-  "wp_annotated_step fs Q \<equiv> (\<forall>fs'. annotated_step fs fs' \<longrightarrow> \<not>is_berr fs' \<and> Q fs')"
+  "wp_annotated_step fs Q \<equiv> (\<forall>fs'. fs \<Rightarrow>\<^sub>f fs' \<longrightarrow> \<not>is_errf fs' \<and> Q fs')"
 
 lemma wp_step_intro:
-  assumes "map_of (llvm_function.blocks f) l = Some b"
+  assumes "map_of (funcs program) f = Some fu"
+  assumes "map_of (llvm_function.blocks fu) l = Some b"
   assumes "wp_instrs
     (execi p b s)
     (\<lambda>s'.
       (case s' of
         (flowi s'' br) \<Rightarrow>
           (case br of
-            branch_label l' \<Rightarrow> Q (bbranch s'' (Some l) l')
-          | return_value v  \<Rightarrow> Q (bret s'' v)
+            branch_label l' \<Rightarrow> Q (branchf s'' (Some l) l' f)
+          | return_value v  \<Rightarrow> Q (retf s'' v f)
           )
       )
     )"
-  shows "wp_step (bbranch s p l) Q"
-    unfolding wp_step_def
-    using assms(1)
+  shows "wp_step (branchf s p l f) Q"
+    using assms
+    unfolding wp_step_def wp_instrs_def
     apply clarsimp
-    subgoal premises prems for fs' s'
-    proof (cases s')
-      case (execi x11 x12 x13)
-      then show ?thesis using prems by simp
-    next
-      case (flowi x21 x22)
+    subgoal premises prems for fs'
+    proof (cases fs')
+      case (branchf x11 x12 x13 x14)
       then show ?thesis
-        using prems apply (auto split: llvm_block_return.splits) using assms(2) unfolding wp_instrs_def by auto  
-        
+        by (smt (verit) function_state.disc function_state.sel instruction_state.simps
+            is_errf_def llvm_block_return.simps option.sel prems step_f.cases term_state_i_simps)
     next
-      case erri
-      then show ?thesis using prems assms
-        using instruction_state.disc(9) wp_instrs_def by blast
+      case (retf x21 x22)
+      then show ?thesis
+        by (smt (verit) function_state.disc function_state.sel instruction_state.simps
+            is_errf_def llvm_block_return.simps option.sel prems step_f.cases term_state_i_simps)
+    next
+      case errf
+      then show ?thesis
+        by (smt (verit) assms function_state.disc instruction_state.disc function_state.inject function_state.sel instruction_state.simps
+            is_errf_def llvm_block_return.simps option.sel prems step_f.cases term_state_i_simps option.distinct)
     qed
     done
 
@@ -800,73 +554,160 @@ lemma wp_steps_until_intro:
 lemma wp_annotated_step_intro:
   assumes "wp_step fs (\<lambda>fs'. wp_steps_until fs' Q)"
   shows "wp_annotated_step fs Q"
-  using assms
+  using assms converse_rtranclpE
   unfolding wp_annotated_step_def wp_step_def annotated_step_def wp_steps_until_def
   by blast
 
 
 
-definition "floyd_cond s p l \<equiv> wp_annotated_step (bbranch s p l) (\<lambda>fs'. annotation_holds fs')"
+definition "floyd_cond s p l f \<equiv> wp_annotated_step (branchf s p l f) (\<lambda>fs'. annotation_holds fs')"
 
 
 definition floyd_vc :: "bool" where
   "floyd_vc \<equiv>
-    map_of annotations (None, first_label) \<noteq> None
-    \<and> (\<forall>p l. map_of annotations (p,l) \<noteq> None \<longrightarrow>
-        (\<forall>s. annotation_holds (bbranch s p l) \<longrightarrow> floyd_cond s p l))"
+    \<forall>f. map_of (funcs program) f \<noteq> None \<longrightarrow> \<comment> \<open>for all functions in our program\<close>
+    first_label (the (map_of (funcs program) f)) \<noteq> None \<and> \<comment> \<open>there is a first block\<close>
+    (case map_of annotations f of
+      None \<Rightarrow> False \<comment> \<open>and there are annotations\<close>
+    | Some (pres,post) \<Rightarrow>
+        (map_of pres (None, the (first_label (the (map_of (funcs program) f)))) \<noteq> None) \<and> \<comment> \<open>and the first block has a precondition\<close>
+        (\<forall>p l. map_of pres (p,l) \<noteq> None \<longrightarrow> \<comment> \<open>and for all annotated blocks\<close>
+          (\<forall>s. annotation_holds (branchf s p l f) \<longrightarrow> floyd_cond s p l f) \<comment> \<open>all states that satisfy the precond will satisfy any following precond\<close>
+        )
+    )"
 
-lemma predicate_for_all_impl_for_all_map_of:
-  assumes "predicate_for_all (\<lambda>p l. (\<forall>s. annotation_holds (bbranch s p l) \<longrightarrow> floyd_cond s p l)) a"
-  shows "(\<forall>p l. map_of a (p,l) \<noteq> None \<longrightarrow> (\<forall>s. annotation_holds (bbranch s p l) \<longrightarrow> floyd_cond s p l))"
+
+fun annotation_holds_list where
+  "annotation_holds_list P [] = True"
+| "annotation_holds_list P (((p,l),pre)#pres) = (P p l \<and> annotation_holds_list P pres)"
+
+lemma annotation_holds_list_imp_annotation_holds:
+  assumes "annotation_holds_list (\<lambda>p l. (\<forall>s. annotation_holds (branchf s p l f) \<longrightarrow> floyd_cond s p l f)) pres"
+  shows "(\<forall>p l. map_of pres (p,l) \<noteq> None \<longrightarrow> \<comment> \<open>and for all annotated blocks\<close>
+          (\<forall>s. annotation_holds (branchf s p l f) \<longrightarrow> floyd_cond s p l f) \<comment> \<open>all states that satisfy the precond will satisfy any following precond\<close>
+        )"
   using assms
-  apply (induction a)
-  subgoal by force
-  subgoal for annot annots
+  apply (induction pres)
+  apply force
+  subgoal for pre pres
     apply (intro allI impI)
     subgoal for p l s
-      apply (cases "annot")
-      subgoal for br pre
+      apply (cases "pre")
+      subgoal for br precond
         apply (cases "br = (p,l)")
         subgoal
-          by (metis (no_types, lifting) predicate_for_all.simps(2))
+          by (metis (no_types, lifting) annotation_holds_list.simps(2))
         subgoal premises prems
         proof -
-          have "predicate_for_all (\<lambda>p l. (\<forall>s. annotation_holds (bbranch s p l) \<longrightarrow> floyd_cond s p l)) annots" using prems
-            using predicate_for_all.elims(2) by blast 
+          have "annotation_holds_list (\<lambda>p l. (\<forall>s. annotation_holds (branchf s p l f) \<longrightarrow> floyd_cond s p l f)) pres"
+            using prems annotation_holds_list.elims(2)
+            by blast 
+          
           then show ?thesis
-            by (metis map_of_Cons_code(2) prems(1,3,4,5,6))
+            using prems map_of_Cons_code(2)
+            by metis
         qed
         done
       done
     done
   done
 
+fun annotations_hold_list :: "(llvm_identifier \<Rightarrow> bool) \<Rightarrow> (llvm_identifier * llvm_function) list \<Rightarrow> bool" where
+  "annotations_hold_list P [] = True"
+| "annotations_hold_list P ((fi,fu)#funs) = (P fi \<and> annotations_hold_list P funs)"
+
+lemma annotations_hold_list_imp_floyd_vc:
+  assumes "annotations_hold_list (\<lambda>f. first_label (the (map_of (funcs program) f)) \<noteq> None \<and> \<comment> \<open>there is a first block\<close>
+    (case map_of annotations f of
+      None \<Rightarrow> False \<comment> \<open>and there are annotations\<close>
+    | Some (pres,post) \<Rightarrow>
+        (map_of pres (None, the (first_label (the (map_of (funcs program) f)))) \<noteq> None) \<and> \<comment> \<open>and the first block has a precondition\<close>
+        (\<forall>p l. map_of pres (p,l) \<noteq> None \<longrightarrow> \<comment> \<open>and for all annotated blocks\<close>
+          (\<forall>s. annotation_holds (branchf s p l f) \<longrightarrow> floyd_cond s p l f) \<comment> \<open>all states that satisfy the precond will satisfy any following precond\<close>
+        )
+    )) funs"
+  shows "\<forall>f. map_of (funs) f \<noteq> None \<longrightarrow> \<comment> \<open>for all functions in our program\<close>
+    first_label (the (map_of (funcs program) f)) \<noteq> None \<and> \<comment> \<open>there is a first block\<close>
+    (case map_of annotations f of
+      None \<Rightarrow> False \<comment> \<open>and there are annotations\<close>
+    | Some (pres,post) \<Rightarrow>
+        (map_of pres (None, the (first_label (the (map_of (funcs program) f)))) \<noteq> None) \<and> \<comment> \<open>and the first block has a precondition\<close>
+        (\<forall>p l. map_of pres (p,l) \<noteq> None \<longrightarrow> \<comment> \<open>and for all annotated blocks\<close>
+          (\<forall>s. annotation_holds (branchf s p l f) \<longrightarrow> floyd_cond s p l f) \<comment> \<open>all states that satisfy the precond will satisfy any following precond\<close>
+        )
+    )"
+  using assms
+  apply (induction funs)
+  apply force
+  subgoal for f fs
+    apply (cases f)
+    apply (intro allI impI)
+    subgoal for fi fu f'
+      apply (cases "fi = f'")
+      subgoal
+        using annotations_hold_list.simps(2) n_lists.simps(2) split_cong option.case_eq_if
+        by (smt (verit))
+      subgoal premises prems
+      proof -
+        have "annotations_hold_list (\<lambda>f. first_label (the (map_of (funcs program) f)) \<noteq> None \<and> \<comment> \<open>there is a first block\<close>
+          (case map_of annotations f of
+            None \<Rightarrow> False \<comment> \<open>and there are annotations\<close>
+          | Some (pres,post) \<Rightarrow>
+            (map_of pres (None, the (first_label (the (map_of (funcs program) f)))) \<noteq> None) \<and> \<comment> \<open>and the first block has a precondition\<close>
+              (\<forall>p l. map_of pres (p,l) \<noteq> None \<longrightarrow> \<comment> \<open>and for all annotated blocks\<close>
+                (\<forall>s. annotation_holds (branchf s p l f) \<longrightarrow> floyd_cond s p l f) \<comment> \<open>all states that satisfy the precond will satisfy any following precond\<close>
+              )
+          )) fs" using prems
+          by (metis (no_types, lifting) annotations_hold_list.simps(2))
+        then show ?thesis
+          using prems(1,3,4,5) by fastforce
+      qed
+      done
+    done
+  done
+
 lemma floyd_vc_intro:
-  assumes "map_of annotations (None, first_label) \<noteq> None"
-  assumes "predicate_for_all (\<lambda>p l. (\<forall>s. annotation_holds (bbranch s p l) \<longrightarrow> floyd_cond s p l)) annotations"
+  assumes "annotations_hold_list (\<lambda>f. first_label (the (map_of (funcs program) f)) \<noteq> None \<and> \<comment> \<open>there is a first block\<close>
+    (case map_of annotations f of
+      None \<Rightarrow> False \<comment> \<open>and there are annotations\<close>
+    | Some (pres,post) \<Rightarrow>
+        (map_of pres (None, the (first_label (the (map_of (funcs program) f)))) \<noteq> None) \<and> \<comment> \<open>and the first block has a precondition\<close>
+        (\<forall>p l. map_of pres (p,l) \<noteq> None \<longrightarrow> \<comment> \<open>and for all annotated blocks\<close>
+          (\<forall>s. annotation_holds (branchf s p l f) \<longrightarrow> floyd_cond s p l f) \<comment> \<open>all states that satisfy the precond will satisfy any following precond\<close>
+        )
+    )) (funcs program)"
   shows "floyd_vc"
+  using assms annotations_hold_list_imp_floyd_vc
   unfolding floyd_vc_def
-  using predicate_for_all_impl_for_all_map_of assms
   by blast
+
 
 lemma floyd_vc_impl_annotation_holds:
   assumes "floyd_vc"
-  shows "\<forall>fs fs'. annotation_holds fs \<and> fs \<Rightarrow> fs' \<longrightarrow> annotation_holds fs'"
-  using assms
-  unfolding floyd_vc_def floyd_cond_def 
-  apply (auto split: flow_state.splits)
-  subgoal for fs fs' a
-    unfolding annotation_holds_def annotated_step_def
-  apply (cases fs)
-    apply force apply force
-    by (metis (no_types, lifting) Steps.floyd_cond_def Steps.floyd_vc_def annotated_step_def
-        annotation_holds_def assms flow_state.case_eq_if flow_state.disc(6) flow_state.sel(4,5) option.simps(4)
-        wp_annotated_step_def)
+  shows "\<forall>fs fs'. annotation_holds fs \<and> fs \<Rightarrow>\<^sub>f fs' \<longrightarrow> annotation_holds fs'"
+  apply (auto split: function_state.splits)
+  subgoal premises prems for fs fs'
+  proof (cases fs)
+    case (branchf s p l f)
+    then show ?thesis
+      using assms prems
+      unfolding floyd_vc_def floyd_cond_def wp_annotated_step_def annotation_holds_def
+      by (smt (verit, ccfv_SIG) case_optionE case_prodE case_prod_conv function_state.simps(9) option.simps(4,5))
+  next
+    case (retf x21 x22 x23)
+    then show ?thesis
+      using annotated_step_def local.term_state_f_simps local.terminal_state_f_def prems
+      by blast
+  next
+    case errf
+    then show ?thesis 
+      using annotated_step_def local.term_state_f_simps local.terminal_state_f_def prems
+      by force 
+  qed
   done
 
-
 lemma floyd_vc_impl_annotated_steps_hold:
-  assumes "fs \<Rightarrow>* fs'"
+  assumes "fs \<Rightarrow>\<^sub>f* fs'"
   assumes "floyd_vc"
   assumes "annotation_holds fs"
   shows "annotation_holds fs'"
@@ -874,9 +715,9 @@ lemma floyd_vc_impl_annotated_steps_hold:
   by (induction rule: converse_rtranclp_induct; blast)
 
 lemma exists_first_cutpoint:
-  assumes "fs \<rightarrow>^n fs'"
-  assumes "is_berr fs' \<or> has_annotation fs'"
-  shows "\<exists>fsp m. step_until\<^sup>*\<^sup>* fs fsp \<and> (is_berr fsp \<or> has_annotation fsp) \<and> fsp \<rightarrow>^m fs' \<and> m \<le> n"
+  assumes "fs \<rightarrow>\<^sub>f^n fs'"
+  assumes "is_errf fs' \<or> has_annotation fs'"
+  shows "\<exists>fsp m. step_until\<^sup>*\<^sup>* fs fsp \<and> (is_errf fsp \<or> has_annotation fsp) \<and> fsp \<rightarrow>\<^sub>f^m fs' \<and> m \<le> n"
   using assms
   proof (induction n arbitrary: fs)
     case 0
@@ -887,17 +728,17 @@ lemma exists_first_cutpoint:
     case (Suc n)
   
     then show ?case
-      by (smt (verit, ccfv_threshold) n_steps.elims(1) nat.inject nat_le_linear not_less_eq_eq
+      by (smt (verit, ccfv_threshold) n_steps_f.elims(1) nat.inject nat_le_linear not_less_eq_eq
           r_into_rtranclp rtranclp.rtrancl_refl rtranclp_trans step_until_def)
   qed
 
 
 lemma steps_to_annotation_impl_annotated_steps:
-  assumes path: "fs \<rightarrow>* fs'"
-  assumes annot: "has_annotation fs' \<or> is_berr fs'"
-  shows "fs \<Rightarrow>* fs'"
+  assumes path: "fs \<rightarrow>\<^sub>f* fs'"
+  assumes annot: "has_annotation fs' \<or> is_errf fs'"
+  shows "fs \<Rightarrow>\<^sub>f* fs'"
 proof -
-  obtain n where ndef: "fs \<rightarrow>^n fs'" using path steps_exists_n_steps by blast
+  obtain n where ndef: "fs \<rightarrow>\<^sub>f^n fs'" using path steps_f_exists_n_steps by blast
   
   then show ?thesis
   proof (induction n arbitrary: fs rule: less_induct)
@@ -910,17 +751,17 @@ proof -
         using less by fastforce
       next
         case (Suc n')
-        then obtain fs1 where fs1def1: "fs \<rightarrow> fs1" and fs1def: "fs1 \<rightarrow>^n' fs'"
+        then obtain fs1 where fs1def1: "fs \<rightarrow>\<^sub>f fs1" and fs1def: "fs1 \<rightarrow>\<^sub>f^n' fs'"
           using less ndef
           by auto
 
-        obtain fsa m where "step_until\<^sup>*\<^sup>* fs1 fsa" "has_annotation fsa \<or> is_berr fsa" "fsa \<rightarrow>^m fs'" "m \<le> n'"
+        obtain fsa m where "step_until\<^sup>*\<^sup>* fs1 fsa" "has_annotation fsa \<or> is_errf fsa" "fsa \<rightarrow>\<^sub>f^m fs'" "m \<le> n'"
           using fs1def exists_first_cutpoint annot
           by blast
 
-      then have "fs \<Rightarrow> fsa" using fs1def1 unfolding annotated_step_def by blast
+      then have "fs \<Rightarrow>\<^sub>f fsa" using fs1def1 unfolding annotated_step_def by blast
 
-      also from less.IH[OF _ \<open>fsa \<rightarrow>^m fs'\<close>] \<open>m \<le> n'\<close> Suc annot have "fsa \<Rightarrow>* fs'" by force
+      also from less.IH[OF _ \<open>fsa \<rightarrow>\<^sub>f^m fs'\<close>] \<open>m \<le> n'\<close> Suc annot have "fsa \<Rightarrow>\<^sub>f* fs'" by force
       
       finally show ?thesis .
       qed
@@ -928,16 +769,76 @@ proof -
   qed
 
 
+lemma function_steps_keep_function:
+  assumes "fs \<rightarrow>\<^sub>f* fs'"
+  assumes "fs = branchf s p l f"
+  shows "(case fs' of retf s' v f' \<Rightarrow> f' = f | branchf s' p' l' f' \<Rightarrow> f' = f | errf \<Rightarrow> True)"
+proof (cases fs')
+  case (branchf s' p' l' f')
+  show ?thesis
+    using assms(1)
+    apply (induction rule: rtranclp_induct)
+    using assms(2)
+     apply simp
+    using local.step_f.cases by fastforce
+next
+  case (retf x21 x22 x23)
+  show ?thesis 
+    using assms(1)
+    apply (induction rule: rtranclp_induct)
+    using assms(2)
+     apply simp
+    using local.step_f.cases by fastforce
+next
+  case errf
+  then show ?thesis
+    by simp
+qed
+
+
 lemma floyd_vc_impl_wp_step:
   assumes "floyd_vc"
+  assumes "map_of (funcs program) f = Some fu"
+  assumes "map_of annotations f = Some (pres,post)"
+  assumes "first_label fu = Some fl"
   assumes "annotation_holds fs"
-  assumes "fs = bbranch s None first_label"
-  shows "wp_steps fs post"
-  using assms 
-  unfolding floyd_vc_def floyd_cond_def wp_steps_def
-  by (metis (no_types, lifting) Steps.annotation_holds_def Steps.has_annotation_def assms(1)
-      flow_state.case_eq_if floyd_vc_impl_annotated_steps_hold steps_to_annotation_impl_annotated_steps
-      terminal_non_err)
+  assumes "fs = branchf s None fl f"
+  shows "wp_func fs post"
+  unfolding wp_func_def
+  apply (intro allI impI)
+  subgoal premises prems for fs'
+  proof -
+    have "has_annotation fs'"
+      unfolding has_annotation_def
+      by (smt (verit, ccfv_SIG) Steps.terminal_non_err annotation_holds_def assms(1,5) floyd_vc_def
+          floyd_vc_impl_annotated_steps_hold function_state.case_eq_if function_state.disc(2) function_state.sel(7)
+          function_state.simps(11) function_state.split_sel_asm is_errf_def le_boolD local.step_f.cases
+          local.term_state_f_simps(3) option.distinct(1) option.simps(4) prems rtranclp.simps
+          steps_to_annotation_impl_annotated_steps)
+    
+    then have "fs \<Rightarrow>\<^sub>f* fs'" using prems steps_to_annotation_impl_annotated_steps
+      by blast
+
+    then have "annotation_holds fs'"
+      using assms(1,5) floyd_vc_impl_annotated_steps_hold by blast
+
+    then show ?thesis
+      using prems
+      unfolding annotation_holds_def
+      apply (cases fs')
+        apply force defer apply force apply (erule conjE)
+      subgoal premises prems' for s v f'
+      proof -
+        have "f = f'" using prems' function_steps_keep_function assms function_state.simps
+          by (smt (verit, ccfv_threshold))
+
+        then show ?thesis
+          using assms prems'
+          by force
+      qed
+      done
+  qed
+  done
 
 end
 
