VCG.thy
@@ -94,11 +94,12 @@ method strat_load_dbg   = rule asm_rl[of "wp (execute_load _ _ _) _"], strat_ins
 method strat_add_dbg    = rule asm_rl[of "wp (execute_add _ _ _ _ _) _"], strat_instr_dbg
 method strat_icmp_dbg   = rule asm_rl[of "wp (execute_icmp _ _ _ _ _ _) _"], strat_instr_dbg
 
-method unfold_block_instr = rule asm_rl[of "wp (execute_block _ ([], _#_, _) _) _"], rule wp_intro
+method unfold_wp_instrs_instr = rule asm_rl[of "wp_instrs _ (execi _ ([],_#_,_) _) _"], rule wp_instrs_intro
+
 method unfold_instr = rule asm_rl[of "wp (execute_instruction _ _) _"], rule wp_intro
 
-method instr_vcg_step = unfold_block_instr | unfold_instr | strat_alloca | strat_store | strat_load | strat_add | strat_icmp
-method instr_vcg_step_dbg = unfold_block_instr | unfold_instr | strat_alloca_dbg | strat_store_dbg | strat_load_dbg | strat_add_dbg | strat_icmp_dbg
+method instr_vcg_step = unfold_wp_instrs_instr | unfold_instr | strat_alloca | strat_store | strat_load | strat_add | strat_icmp
+method instr_vcg_step_dbg = unfold_wp_instrs_instr | unfold_instr | strat_alloca_dbg | strat_store_dbg | strat_load_dbg | strat_add_dbg | strat_icmp_dbg
 
 
 subsection "Phi Node Methods"
@@ -106,53 +107,56 @@ subsection "Phi Node Methods"
 method strat_phi = rule asm_rl[of "wp (execute_phi _ _ _) _"], strat_instr \<open>sub_distinct_first, sub_some_refl, sub_map_of_some, sub_register_value\<close>
 method strat_phi_dbg = rule asm_rl[of "wp (execute_phi _ _ _) _"], strat_instr_dbg
 
-method unfold_block_phi = rule asm_rl[of "wp (execute_block _ (_#_, _, _) _) _"], rule wp_intro
+method unfold_wp_instrs_phi = rule asm_rl[of "wp_instrs _ (execi _ (_#_,_,_) _) _"], rule wp_instrs_intro
 
-method phi_vcg_step = unfold_block_phi | strat_phi
-method phi_vcg_step_dbg = unfold_block_phi | strat_phi_dbg
+method phi_vcg_step = unfold_wp_instrs_phi | strat_phi
+method phi_vcg_step_dbg = unfold_wp_instrs_phi | strat_phi_dbg
 
 
 subsection "Terminal Instruction Methods"
 
-(*
-method strat_branch_i1 = rule asm_rl[of "wp (execute_block _ ([], [], br_i1 _ _ _) _ ) _"], (rule wp_intro, sub_register_value); (simp only: False_eq_False)?
-method strat_branch_label = rule asm_rl[of "wp (execute_block _ ([], [], br_label _) _ ) _"], rule wp_intro; (simp only: False_eq_False)?
-method strat_return = rule asm_rl[of "wp (execute_block _ ([], [], ret _ _) _ ) _"], (rule wp_intro, sub_register_value); (simp only: False_eq_False)?
 
-method term_vcg_step_dbg = rule asm_rl[of "wp (execute_block _ ([], [], _) _) _"], rule wp_intro, (solve_subgoal+)?; (simp only: False_eq_False)?
+method strat_branch_i1 = rule asm_rl[of "wp_instrs _ (execi _ ([], [], br_i1 _ _ _) _) _"], (intro wp_instrs_intro, sub_register_value); (simp only: False_eq_False)?
+method strat_branch_label = rule asm_rl[of "wp_instrs _ (execi  _ ([], [], br_label _) _ ) _"], intro wp_instrs_intro; (simp only: False_eq_False)?
+method strat_return = rule asm_rl[of "wp_instrs _ (execi _ ([], [], ret _) _ ) _"], (intro wp_instrs_intro, sub_register_value); (simp only: False_eq_False)?
 
 method term_vcg_step = strat_branch_i1 | strat_branch_label | strat_return
-*)
+method term_vcg_step_dbg = rule asm_rl[of "wp_instrs _ (execi _ ([], [], _) _) _"], intro wp_instrs_intro, (solve_subgoal+)?; (simp only: False_eq_False)?
+
 
 subsection "Block VCG Methods"
 
-method unfold_wp_instrs = rule asm_rl[of "wp_instrs _ _"], rule wp_instrs_intro
+method block_vcg_step = phi_vcg_step | instr_vcg_step | term_vcg_step
+method block_vcg_step_dbg = phi_vcg_step_dbg | instr_vcg_step_dbg | term_vcg_step_dbg
 
-method block_vcg_step = unfold_wp_instrs | phi_vcg_step | instr_vcg_step
-method block_vcg_step_dbg = unfold_wp_instrs | phi_vcg_step_dbg | instr_vcg_step_dbg
-
-method block_vcg uses pres blocks = (subst (asm) pres)?, (subst blocks)?, unfold_unique_addresses?, block_vcg_step+, (simp (no_asm))?, \<comment> \<open>branching\<close>(intro conjI impI)?
-method block_vcg_dbg uses pres blocks = (subst (asm) pres)?, (subst blocks)?, unfold_unique_addresses?, block_vcg_step_dbg+, (simp (no_asm))?, (intro conjI impI)?
+method block_vcg uses pres blocks = (subst (asm) pres)?, (subst (2) blocks)?, unfold_unique_addresses?, block_vcg_step+; (simp (no_asm))?, (intro conjI impI)?
+method block_vcg_dbg uses pres blocks = (subst (asm) pres)?, (subst (2) blocks)?, unfold_unique_addresses?, block_vcg_step_dbg+, (simp (no_asm))?, (intro conjI impI)?
 
 
 subsection "Multi-Block VCG Methods"
 
-method unfold_floyd_vc uses defs =
-  rule asm_rl[of "floyd_vc _ _ _"],
+method unfold_floyd uses prog_def func_def =
+  rule asm_rl[of "floyd_vc _ _"],
   rule floyd_vc_intro,
-  unfold defs,
-  (unfold first_label_def; simp; fail)?,
-  simp only: predicate_for_all.simps HOL.simp_thms(21),
-  (intro conjI allI impI; unfold annotation_holds_def has_annotation_def; simp; unfold floyd_cond_def)
+  unfold first_label_def floyd_cond_def annotation_holds_def has_annotation_def,
+  (simp add: prog_def),
+  intro conjI allI impI;
+  (simp add: func_def)?;
+  ((thin_tac "_ = Some (lid _)" | thin_tac "_ = None"), simp only: triv_forall_equality)?
 
-method instantiate_block_def =
-  rule asm_rl[of "map_of _ _ = Some _"],
+
+method instantiate_block =
+  rule asm_rl[of "map_of _ (lid _) = Some _"],
+  force
+method instantiate_func =
+  rule asm_rl[of "map_of _ (gid _) = Some _"],
   force
 
 method unfold_wp_step =
   rule asm_rl[of "wp_step _ _ _"],
   rule wp_step_intro,
-  instantiate_block_def
+  instantiate_func,
+  instantiate_block
 
 method unfold_wp_annotated_step =
   rule asm_rl[of "wp_annotated_step _ _ _ _"],
@@ -170,12 +174,8 @@ method unfold_wp_steps_until =
   rule asm_rl[of "wp_steps_until _ _ _ _"],
   rule wp_steps_until_intro;
   (unfold has_annotation_def; force; fail)?;
-  (thin_tac "\<not>has_annotation _ _" | thin_tac "has_annotation _ _")?;
+  (thin_tac "\<not>has_annotation _ _ _" | thin_tac "has_annotation _ _ _")?;
   (unfold_wp_step | unfold_endgoal)?
-
-
-method clean_goal' = (simp (no_asm_simp) split: prod.splits del: register_\<alpha>.simps registers_contain_unique_addresses.simps, intro allI conjI impI)
-method clean_goal = (match conclusion in "case _ of (s, r) \<Rightarrow> (case r of return_value _ \<Rightarrow> _ | branch_label _ \<Rightarrow> _)" \<Rightarrow> clean_goal')
 
 
 end
